src/program_proof/txn/recovery_proof.v
@@ -1,0 +1,29 @@
+From Perennial.Helpers Require Import Transitions NamedProps Map.
+From Perennial.program_proof Require Import proof_prelude.
+From Perennial.algebra Require Import auth_map log_heap.
+
+From Goose.github_com.mit_pdos.goose_nfsd Require Import txn.
+From Goose.github_com.mit_pdos.goose_nfsd Require Import wal.
+From Perennial.program_proof Require Import wal.specs wal.lib wal.heapspec addr.addr_proof buf.buf_proof disk_lib.
+From Perennial.program_proof Require Import txn.invariant.
+From Perennial.goose_lang.lib Require Import slice.typed_slice.
+
+Section goose_lang.
+Context `{!txnG Σ}.
+
+(* TODO: set up crash_obligation_alt for txn *)
+
+(* Definitely missing the durable invariant of the heapspec layer, which should
+say something more complete about [γ.(txn_walnames)]. Otherwise there probably
+isn't enough to relate the state inside [is_txn_always] to that in
+[is_wal_inner_durable]. *)
+Theorem wp_MkTxn (d:loc) σ dinit (γ:txn_names) :
+  {{{ is_wal_inner_durable γ.(txn_walnames).(wal_heap_walnames) σ dinit ∗
+      is_txn_always γ
+  }}}
+    MkTxn #d
+  {{{ (l: loc) (γ':txn_names), RET #l; is_txn l γ' dinit }}}.
+Proof.
+Admitted.
+
+End goose_lang.
