src/program_proof/txn/txn_proof.v
@@ -1,2 +1,2 @@
 From Perennial.program_proof.txn Require Export
-     invariant load_proof commit_proof.
+     invariant load_proof commit_proof recovery_proof.
